Final form of quality and paradigm

ImperativeReasoning.thy
@@ -4,18 +4,65 @@ imports AutoCorres.AutoCorres
 
 begin
 
-install_C_file "/Users/alexweisberger/code/recur_finance/test.c"
-autocorres "/Users/alexweisberger/code/recur_finance/test.c"
-print_theorems
+install_C_file "/Users/alexweisberger/code/concerning_quality/test.c"
+autocorres[heap_abs_syntax] "/Users/alexweisberger/code/concerning_quality/test.c"
 
 context test begin
 
 thm update_arr'_def
+thm main'_def
 
-theorem 
-  shows "valid (\<lambda>s :: idk. is_valid_w32 s a) (update_arr' a v) (\<lambda>rv s. is_valid_w32 s a)"
-  unfolding update_arr'_def
+value "array_addrs (PTR(32 word) (symbol_table ''c'')) 3"
+
+definition "array_mem_valid s a = (is_valid_w32 s a \<and> is_valid_w32 s (ptr_add a 1))"
+
+theorem
+  "valid
+    (\<lambda>s. array_mem_valid s a)
+    (update_arr' a v)
+    (\<lambda>_ s. (array_mem_valid s a) \<and> s[ptr_add a 1] = v)"
+  unfolding update_arr'_def and array_mem_valid_def
   apply(wp)
-  apply(auto)
+  apply(auto simp: fun_upd_def)
   done
+
+theorem
+  "valid
+    (\<lambda>s. array_mem_valid s a \<and> s = s0)
+    (update_arr' a v)
+    (\<lambda>_ s. (array_mem_valid s a) \<and> s = s0[(ptr_add a 1) := v])"
+  unfolding update_arr'_def and array_mem_valid_def
+  apply(wp)
+  apply(auto simp: fun_upd_def)
+  done
+
+(* Main is also valid *)
+
+find_theorems is_valid_w32
+
+theorem
+  "validNF
+    (\<lambda>s. True)
+    main'
+    (\<lambda>_ s. True)"
+  unfolding update_arr'_def and main'_def
+  apply(wp)
+   apply(auto simp: fun_upd_def)
+  oops
+
+
+theorem
+  "validNF
+    (\<lambda>s. array_mem_valid s a)
+    (update_arr' a v)
+    (\<lambda>_ s. (array_mem_valid s a) \<and> s[ptr_add a 1] = v)"
+  unfolding update_arr'_def and array_mem_valid_def
+  apply(wp)
+  apply(simp add: fun_upd_def)
+  done
+
+(* theorem - array access is never out of bounds *)
+
+end
+
 end
