ExecutionReasoning.thy
@@ -1,0 +1,32 @@
+theory ExecutionReasoning
+
+imports AutoCorres.AutoCorres
+
+begin
+
+install_C_file "/Users/alexweisberger/code/concerning_quality/response_cache.c"
+autocorres[heap_abs_syntax] "/Users/alexweisberger/code/concerning_quality/response_cache.c"
+                  
+print_theorems
+
+context response_cache begin
+
+
+thm request_data'_def
+
+value "lifted_globals"
+thm request_data'_def
+thm order_from_server'_def
+
+(* Data is only fetched if it isn't already present in the cache *)
+(* theorem "request_data' *)
+
+theorem 
+  "valid 
+    (\<lambda>s. True) 
+    (request_data' i)
+    (\<lambda>rv s. rv = order_from_server' i)"
+
+end
+
+end
